code/streaming/Hacl.Streaming.MD5.fst
@@ -44,4 +44,4 @@ let free = F.free hacl_md5 (G.hide ()) (state_t_md5.s ()) (G.erased unit)
 
 let copy = F.copy hacl_md5 () (state_t_md5.s ()) (G.erased unit)
 
-let hash: Hacl.Hash.Definitions.hash_st MD5 = fun output input input_len -> Hacl.Hash.MD5.hash output input input_len
+let hash: Hacl.Hash.Definitions.hash_st MD5 = fun output input input_len -> Hacl.Hash.MD5.hash_oneshot output input input_len
