code/hash/Hacl.Hash.MD5.fsti
@@ -7,4 +7,4 @@ include Hacl.Hash.Core.MD5
 
 val update_multi: update_multi_st (|MD5, ()|)
 val update_last: update_last_st (|MD5, ()|)
-val hash: hash_st MD5
+val hash_oneshot: hash_st MD5
